theories/L6_PCPS/Ensembles_util.v
@@ -111,7 +111,7 @@ Hint Immediate Same_set_refl Included_refl : Ensembles_DB.
 (** * Decidability  instances *)
 
 Class Decidable {A} (S : Ensemble A) : Type :=
- { Dec : forall x, { S x } + {~ S x} }.
+ { Dec : forall x, { S x  } + {~ S x} }.
 
 Instance Decidable_Union {A} (S1 S2 : Ensemble A)
          {H1 : Decidable S1} {H2 : Decidable S2} : Decidable (Union A S1 S2).
@@ -808,6 +808,23 @@ Proof.
   inv H1. eapply Hd; eauto.
 Qed.
 
+Lemma Union_Same_set_Disjoint {A} (S1 S2 S3 : Ensemble A) :
+  S1 :|: S2 <--> S1 :|: S3 ->
+  Disjoint _ S1 S2 ->
+  Disjoint _ S1 S3 ->
+  S2 <--> S3.
+Proof.
+  intros Heq HD HD'. split; intros x Hin.
+  - assert (Hin' : (S1 :|: S3) x).
+    { eapply Heq. now right. }
+    inv Hin'; eauto.
+    exfalso. eapply HD; eauto.
+  - assert (Hin' : (S1 :|: S2) x).
+    { eapply Heq. now right. }
+    inv Hin'; eauto.
+    exfalso. eapply HD'; eauto.
+Qed.
+
 
 Hint Resolve Disjoint_Setminus_l Disjoint_Setminus_r Union_Disjoint_l
      Union_Disjoint_r Disjoint_Singleton_l Disjoint_Singleton_r
@@ -1353,7 +1370,6 @@ Proof.
     eassumption.
     eexists. split; eauto. now right.
 Qed.
-
 
 Hint Immediate FromList_nil FromList_cons FromList_app
      FromList_singleton : Ensembles_DB.
