theories/L6_PCPS/functions.v
@@ -271,7 +271,6 @@ Proof with now eauto with Ensembles_DB.
   - rewrite !FromList_cons, image_Union, image_Singleton...
 Qed.
 
-
 (** * Lemmas about [extend] *)
 
 Instance extend_Proper {A} : Proper (f_eq ==> Logic.eq ==> Logic.eq ==> f_eq) (@extend A).
@@ -704,6 +703,15 @@ Proof.
     intros Hc; inv Hc; subst; congruence.
 Qed.
 
+Lemma injective_subdomain_extend_r {A} (S : Ensemble positive)  f x (y : A) : 
+  injective_subdomain S (f { x ~> y }) ->
+  injective_subdomain (S \\ [set x]) f.
+Proof.
+  intros Hinj x1 x2 Hin1 Hin2 Heq. inv Hin1; inv Hin2. 
+  eapply Hinj; try eassumption.
+  rewrite !extend_gso; eauto; intros Hc; subst; eauto.  
+Qed.
+
 Lemma injective_subdomain_extend_lst S f xs xs' :
   injective_subdomain (Setminus _ S (FromList xs)) f ->
   Disjoint positive (image f (Setminus positive S (FromList xs))) (FromList xs') ->
@@ -741,6 +749,16 @@ Proof.
   eexists; split; [| reflexivity ]; eauto.
 Qed.
 
+Lemma extend_lst_id f l x :
+  List.In x l ->
+  f <{ l ~> l }> x = x.
+Proof.
+  induction l; intros Hin. 
+  - inv Hin.
+  - inv Hin. simpl.
+    rewrite extend_gss. reflexivity.
+    simpl. unfold extend. destruct (peq x a); eauto.
+Qed.
 
 Lemma injective_extend (f : positive -> positive) x y :
   injective f ->
@@ -767,6 +785,70 @@ Proof.
   intros Hinj. constructor; intros x Hin. inv Hin. 
   destruct H0 as [y [Hin Heq]]. destruct H1 as [y' [Hin' Heq']].
   subst. eapply Hinj in Heq'; eauto. eapply H. subst; eauto.
+Qed.
+
+Lemma FromList_image_exists {A B} (f : A -> B) l S :
+  FromList l \subset image f S ->
+  exists l', l = map f l'.
+Proof with (now eauto with Ensembles_DB).
+  revert S; induction l; intros S Heq; eauto.
+  - eexists []. reflexivity.
+  - rewrite FromList_cons in Heq.
+    edestruct IHl as [l' Heql'].
+    + eapply Included_trans; try eassumption...
+    + edestruct Heq as [a' [Heqa Hina]]. now left.
+      eexists (a' :: l'). simpl; f_equal; eauto.
+Qed.
+
+
+Lemma FromList_image_injective_exists (f : positive -> positive) l S :
+  FromList l <--> image f S ->
+  injective_subdomain S f ->
+  exists l', l = map f l' /\ FromList l' <--> S.
+Proof with (now eauto with Ensembles_DB).
+  revert S; induction l; intros S Heq Hinj; eauto.
+  - eexists []. split; eauto.
+    rewrite !FromList_nil in Heq.
+    rewrite FromList_nil.
+    split; intros x Hin; try now inv Hin.
+    assert (Hc : Empty_set _ (f x)). 
+    { eapply Heq. eexists; split; eauto. }
+    inv Hc. 
+  - rewrite FromList_cons in Heq.
+    assert (Ha : image f S a).
+    { eapply Heq; now left. }
+    destruct Ha as [a' [Heqa Hina]]. subst.
+    
+    destruct (Decidable_FromList l) as [Decl].
+    destruct (Decl (f a')).
+    + rewrite Union_Same_set in Heq; 
+        [| eapply Singleton_Included; now eauto ].  
+      edestruct IHl as [l' [Heql Heqs]]; eauto.
+      subst.
+      eexists (a' :: l'). split. now simpl; f_equal; eauto.
+      rewrite FromList_cons.
+      rewrite Union_Same_set. eassumption.
+      rewrite Heqs. eapply Singleton_Included. eassumption.
+    + assert (Heq' := Heq).
+      rewrite (Union_Setminus_Same_set S [set a']) in Heq;
+        [| eapply Singleton_Included; now eauto ].  
+      rewrite image_Union, image_Singleton in Heq.
+      eapply Union_Same_set_Disjoint in Heq.
+      * edestruct IHl as [l' [Heql Heqs]]; try now apply Heq; eauto; subst.
+        eapply injective_subdomain_antimon; try eassumption...
+        
+        eexists (a' :: l'). split. now simpl; f_equal; eauto.
+        rewrite FromList_cons.
+        rewrite Heqs.
+        rewrite <- (Union_Setminus_Same_set S [set a']);
+          [| eapply Singleton_Included; now eauto ].
+        reflexivity.
+      * eapply Disjoint_Singleton_l. eauto.
+      * rewrite <- image_Singleton.
+        eapply injective_subdomain_Union_not_In_image.
+        eapply injective_subdomain_antimon; try eassumption...
+        eapply Disjoint_Singleton_l.
+        intros Hc; inv Hc; eauto.
 Qed.
 
 (** * Lemmas about [domain] *)
